update

Library/Model/Model.dfy
@@ -18,10 +18,22 @@ module Model {
     Monad.Deconstruct(s)
   }
 
-  function UniformPowerOfTwoModel(n: nat, k: nat := 1, u: nat := 0): Hurd<nat> 
+  function UniformPowerOfTwoModelAlternative(n: nat, k: nat := 1, u: nat := 0): Hurd<nat> 
     requires k >= 1
   {
     (s: RNG) => Unif.ProbUnifAlternative(n, s, k, u)
+  }
+
+  function UniformPowerOfTwoModel(n: nat): (f: Hurd<nat>)
+    ensures forall s :: f(s) == UniformPowerOfTwoModelAlternative(n)(s)
+  {
+    var f := Unif.ProbUnif(n);
+    assert forall s :: f(s) == UniformPowerOfTwoModelAlternative(n)(s) by {
+      forall s ensures f(s) == UniformPowerOfTwoModelAlternative(n)(s) {
+        ProbUnifCorrespondence(n, s);
+      }
+    }
+    f
   }
 
   function UniformModel(n: nat): Hurd<nat> 
