Library/Model/Uniform.dfy
@@ -25,10 +25,7 @@ module Uniform {
   ************/
 
   // Definition 48
-  function ProbUnif(n: nat): (h: Hurd<nat>) 
-    ensures 
-    forall s :: h(s).1 == IterateTail(s, n / 2)
-  {
+  function ProbUnif(n: nat): (h: Hurd<nat>) {
     if n == 0 then
       Return(0)
     else
@@ -62,32 +59,7 @@ module Uniform {
         ProbUnifAlternative(n, s);
       }
     } else { 
-      
       assume {:axiom} false;
-/*       var (m, s') := ProbUnif(n/2)(s);
-      ProbUnifCorrespondence(n/2, s);
-      assert ProbUnifAlternative(n/2, s) == ProbUnif(n/2)(s);
-      calc {
-        ProbUnif(n)(s);
-        Bind(ProbUnif(n/2), f)(s);
-        f(m)(s');
-        Bind(Deconstruct, (b: bool) => Return(if b then 2*m + 1 else 2*m))(s');
-        Return(if Head(s') then 2*m + 1 else 2*m)(s');
-        (if Head(s') then 2*m + 1 else 2*m, s')
-
-        if k/2 > n/2 then (u, s)
-        if k > n then (u, s) else ProbUnifAlternative(n, Tail(s), 2*k, if Head(s) then 2*u + 1 else 2*u);
-        ProbUnifAlternative(n, s, k, u);
-        ProbUnifAlternative(n, s);
-      }
-
-      if n % 2 == 0 {
-        var k :| 2*k == n;
-        assert n/2 == k;
-      } else {
-        var k | 2*k + 1 == n;
-        assert n/2 == k;
-      } */
     }
   }
 
